Monotonicity of the resolution operator

games/HComp.v
@@ -260,8 +260,8 @@ Module Res.
   Section ATS.
     Context {G S K} (α : ats G G S K).
 
-    Definition state : Type := S * list bool.
-    Definition cont : Type := K * list bool.
+    Definition state : Type := S * list player.
+    Definition cont : Type := K * list player.
 
     Inductive step : state -> state -> Prop :=
       | step_int s s' stk :
@@ -270,11 +270,11 @@ Module Res.
       | step_q (m : question G) s k s' stk :
           ATS.suspend α s (pq m, k) ->
           ATS.resume α k (oq m) s' ->
-          step (s, stk) (s', true :: stk)
+          step (s, stk) (s', P :: stk)
       | step_a (m : answer G) s k s' stk :
           ATS.suspend α s (pa m, k) ->
           ATS.resume α k (oa m) s' ->
-          step (s, true :: stk) (s', stk).
+          step (s, P :: stk) (s', stk).
 
     Inductive suspend : state -> pmove G G * cont -> Prop :=
       | suspend_q (m : question G) s k stk :
@@ -283,12 +283,12 @@ Module Res.
           suspend (s, stk) (pq m, (k, stk))
       | suspend_a (m : answer G) s k stk :
           ATS.suspend α s (pa m, k) ->
-          suspend (s, false :: stk) (pa m, (k, stk)).
+          suspend (s, O :: stk) (pa m, (k, stk)).
 
     Inductive resume : cont -> omove G G -> state -> Prop :=
       | resume_q m k s stk :
           ATS.resume α k (oq m) s ->
-          resume (k, stk) (oq m) (s, false :: stk)
+          resume (k, stk) (oq m) (s, O :: stk)
       | resume_a m k s stk :
           ATS.resume α k (oa m) s ->
           resume (k, stk) (oa m) (s, stk).
@@ -302,4 +302,184 @@ Module Res.
       ATS.Build_ats G G state cont step suspend resume refuse.
 
   End ATS.
+
+  Arguments state : clear implicits.
+  Arguments cont : clear implicits.
+
+  Section SIM.
+    Context {G1 G2} (GR : grel G1 G2).
+    Context {S1 S2} (RS : klr (gworld GR GR) S1 S2).
+    Context {K1 K2} (RK : klr (gworld GR GR) K1 K2).
+
+    Inductive extw : bool -> list player -> gworld GR GR -> gworld GR GR -> Prop :=
+      | extw_nil pp :
+          extw false pp nil nil
+      | extw_ext pp w ws ws' :
+          extw false pp ws ws' ->
+          extw true (O::pp) (inr w :: ws) (inr w :: ws')
+      | extw_int pp w ws ws' :
+          extw true pp ws ws' ->
+          extw true (P::pp) (inr w :: inl w :: ws) ws'
+      | extw_dom b pp w ws ws' :
+          extw (negb b) pp ws ws' ->
+          extw b pp (inl w :: ws) (inl w :: ws').
+
+    Inductive state_rel : klr (gworld GR GR) (state S1) (state S2) :=
+      state_rel_intro pp ws ws' s1 s2 :
+        extw true pp ws ws' ->
+        RS ws s1 s2 ->
+        state_rel ws' (s1, pp) (s2, pp).
+
+    Inductive cont_rel : klr (gworld GR GR) (cont K1) (cont K2) :=
+      cont_rel_intro pp ws ws' k1 k2 :
+        extw false pp ws ws' ->
+        RK ws k1 k2 ->
+        cont_rel ws' (k1, pp) (k2, pp).
+  End SIM.
+
+  Global Instance step_sim :
+    Monotonic
+      (@step)
+      (forallr GR, forallr RS, forallr RK,
+        ATS.sim GR GR RS RK ++>
+        |= state_rel GR RS ++> k1 set_le (state_rel GR RS)).
+  Proof.
+    intros G1 G2 GR S1 S2 RS K1 K2 RK.
+    intros α1 α2 Hα ws s1 s2 Hs s1' Hs1'.
+    destruct Hs1' as
+      [s1 s1' stk Hs1' | q1 s1 k1 s1' stk Hk1 Hs1' | a1 s1 k1 s1' stk Hk1 Hs1'];
+    inversion Hs; clear Hs; subst.
+    - (* internal step *)
+      edestruct @ATS.sim_step as (s2' & Hs2' & Hs'); eauto.
+      exists (s2', stk). split.
+      + constructor; auto.
+      + econstructor; eauto.
+    - (* internal question *)
+      edestruct @ATS.sim_suspend as ([m2 k2] & Hqk2 & Hqk); eauto.
+      destruct Hqk as (ws'' & Hq & Hk).
+      apply FComp.gacc_inv_pq in Hq as (w & q2 & Hm2 & Hq & Hws''); subst.
+      inversion Hm2; clear Hm2; subst.
+      edestruct @ATS.sim_resume as (s2 & Hs2 & Hs); eauto.
+      + instantiate (1 := inr w :: inl w :: ws0).
+        instantiate (1 := oq q2).
+        repeat econstructor; auto.
+      + exists (s2, P :: stk). split.
+        * econstructor; eauto.
+        * repeat econstructor; eauto.
+    - (* internal answer *)
+      edestruct @ATS.sim_suspend as ([m2 k2] & Hqk2 & Hqk); eauto.
+      destruct Hqk as (ws'' & Hq & Hk).
+      apply FComp.gacc_inv_pa in Hq as (w & a2 & Hm2 & Ha & Hws''); subst.
+      inversion Hm2; clear Hm2; subst.
+      inversion H2; clear H2; subst.
+      edestruct @ATS.sim_resume as (s2 & Hs2 & Hs); eauto.
+      + instantiate (1 := ws0).
+        instantiate (1 := oa a2).
+        repeat constructor; auto.
+      + exists (s2, stk). split.
+        * econstructor; eauto.
+        * repeat econstructor; eauto.
+  Qed.
+
+  Global Instance suspend_sim :
+    Monotonic
+      (@suspend)
+      (forallr GR, forallr RS, forallr RK,
+        ATS.sim GR GR RS RK ++>
+        |= state_rel GR RS ++> k1 set_le (<> * cont_rel GR RK)).
+  Proof.
+    intros G1 G2 GR S1 S2 RS K1 K2 RK α1 α2 Hα.
+    intros ws s1 s2 Hs km1 Hkm1.
+    destruct Hkm1 as [m1 s1 k1 stk Hsk1 Hkm1 | m1 s1 k1 stk Hmk1];
+    inversion Hs; clear Hs; subst.
+    - (* external P question *)
+      edestruct @ATS.sim_suspend as ([m2 k2] & Hkm2 & Hkm); eauto.
+      destruct Hkm as (ws'' & Hws'' & Hkm).
+      apply FComp.gacc_inv_pq in Hws'' as (w & q2 & Hm2 & Hq & Hws''); subst.
+      inversion Hm2; clear Hm2; subst.
+      exists (pq q2, (k2, stk)). split.
+      + constructor; auto.
+        eapply ATS.sim_refuse; eauto.
+        repeat econstructor; eauto.
+      + exists (inl w :: ws). split.
+        * repeat constructor; auto.
+        * repeat econstructor; eauto.
+    - (* external P answer *)
+      edestruct @ATS.sim_suspend as ([m2 k2] & Hkm2 & Hkm); eauto.
+      destruct Hkm as (ws'' & Hws'' & Hkm).
+      apply FComp.gacc_inv_pa in Hws'' as (w & a2 & Hm2 & Ha & Hws''); subst.
+      inversion Hm2; clear Hm2; subst.
+      inversion H2; clear H2; subst.
+      exists (pa a2, (k2, stk)). split.
+      + constructor; auto.
+      + exists ws'. split.
+        * repeat constructor; auto.
+        * repeat econstructor; eauto.
+  Qed.
+
+  Global Instance resume_sim :
+    Monotonic
+      (@resume)
+      (forallr GR, forallr RS, forallr RK,
+       ATS.sim GR GR RS RK ++>
+       |= cont_rel GR RK ++> ([] -> k1 set_le (state_rel GR RS))).
+  Proof.
+    intros G1 G2 GR S1 S2 RS K1 K2 RK.
+    intros α1 α2 Hα ws k1 k2 Hk m1 m2 ws' Hm s1 Hs1.
+    destruct Hs1 as [q1 k1 s1 stk Hs1 | a1 k1 s1 stk Hs1];
+    inversion Hk; clear Hk; subst;
+    inversion Hm; clear Hm; subst.
+    - (* external O question *)
+      inversion H5; clear H5; subst.
+      edestruct @ATS.sim_resume as (s2 & Hs2 & Hs); eauto.
+      + instantiate (1 := inr w0 :: ws0).
+        instantiate (1 := oq m0).
+        repeat constructor; auto.
+      + exists (s2, O :: stk). split.
+        * constructor; auto.
+        * repeat econstructor; eauto.
+    - inversion H5.
+    - inversion H5.
+    - (* external O answer *)
+      inversion H5; clear H5; subst.
+      inversion H2; clear H2; subst.
+      edestruct @ATS.sim_resume as (s2 & Hs2 & Hs); eauto.
+      + instantiate (1 := ws).
+        instantiate (1 := oa m0).
+        repeat constructor; auto.
+      + exists (s2, stk). split.
+        * constructor; auto.
+        * repeat econstructor; eauto.
+  Qed.
+
+  Global Instance refuse_sim :
+    Monotonic
+      (@refuse)
+      (forallr GR, forallr RS, forallr RK,
+       ATS.sim GR GR RS RK ++>
+       |= cont_rel GR RK ++> ([] -> k impl)).
+  Proof.
+    intros G1 G2 GR S1 S2 RS K1 K2 RK.
+    intros α1 α2 Hα ws k1 k2 Hk m1 m2 ws' Hm Hm1.
+    destruct Hm1;
+    inversion Hk; clear Hk; subst;
+    inversion Hm; clear Hm; subst;
+    inversion H6; clear H6; subst.
+    constructor.
+    eapply ATS.sim_refuse, H; eauto.
+    instantiate (1 := inr w0 :: ws0).
+    repeat constructor; auto.
+  Qed.
+
+  Global Instance of_sim :
+    Monotonic
+      (@of)
+      (forallr GR, forallr RS, forallr RK,
+       ATS.sim GR GR RS RK ++>
+       ATS.sim GR GR (state_rel GR RS) (cont_rel GR RK)).
+  Proof.
+    intros G1 G2 GR S1 S2 RS K1 K2 RK α1 α2 H.
+    split; simpl; rauto.
+  Qed.
+
 End Res.
